Rename Sequence.Length() => Cardinality()

Source/DafnyCore/DafnyOptions.cs
@@ -675,18 +675,6 @@ namespace Microsoft.Dafny {
     public override void ApplyDefaultOptions() {
       base.ApplyDefaultOptions();
 
-      // We check that we haven't already set BoogieXmlFilename here
-      // so that we don't hit spurious errors or generate another temporary file name
-      // when cloning options.
-      if (VerificationLoggerConfigs.Any() && BoogieXmlFilename == null) {
-        if (XmlSink != null) {
-          throw new Exception("The /verificationLogger and /xml options cannot be used at the same time.");
-        }
-
-        BoogieXmlFilename = Path.GetTempFileName();
-        XmlSink = new Bpl.XmlSink(this, BoogieXmlFilename);
-      }
-
       Compiler ??= new CsharpCompiler();
 
       // expand macros in filenames, now that LogPrefix is fully determined
